src/program_proof/mvcc/mvcc_inv.v
@@ -1,11 +1,6 @@
 From Perennial.program_proof.mvcc Require Import mvcc_prelude.
 From Perennial.program_proof.mvcc Require Import mvcc_ghost mvcc_misc mvcc_action mvcc_tuplext proph_proof.
 
-(* Invariant namespaces. *)
-Definition mvccN := nroot .@ "mvcc".
-Definition mvccNSST := mvccN .@ "sst".
-Definition mvccNGC := mvccN .@ "gc".
-
 Section def.
 Context `{!heapGS Σ, !mvcc_ghostG Σ}.
 
@@ -14,7 +9,7 @@ Definition mvcc_inv_gc_site_def γ (sid : u64) : iProp Σ :=
   ∃ (tids : gset nat) (tidmin tidmax : nat),
     "HactiveA" ∷ site_active_tids_half_auth γ sid tids ∗
     "HminA"    ∷ site_min_tid_auth γ sid tidmin ∗
-    "#Htslb"   ∷ ts_lb γ (S tidmax) ∗
+    "#Htslb"   ∷ ts_lb γ tidmax ∗ (* Ralf changed this and had no idea if that makes any sense *)
     "%Hmin"    ∷ ⌜set_Forall (λ tid, tidmin ≤ tid)%nat tids⌝ ∗
     "%Hmax"    ∷ ⌜set_Forall (λ tid, tid ≤ tidmax)%nat ({[ tidmin ]} ∪ tids)⌝.
 
