src/program_proof/mvcc/txn_begin.v
@@ -12,11 +12,11 @@ Context `{!heapGS Σ, !mvcc_ghostG Σ}.
 Theorem wp_txn__begin txn γ :
   ⊢ {{{ own_txn_uninit txn γ }}}
     <<< ∀∀ (ts : nat), ts_auth γ ts >>>
-      Txn__begin #txn @ ↑mvccNGC
-    <<< ∃ ts', ts_auth γ ts' ∗ ⌜(ts < ts')%nat⌝ >>>
+      Txn__begin #txn @ ↑mvccNGC ∪ ↑mvccNTID
+    <<< ∃∃ ts', ts_auth γ ts' ∗ ⌜(ts < ts')%nat⌝ >>>
     {{{ (tid : u64) (wrbuf : loc), RET #();
-        own_txn_impl txn wrbuf ts γ ∗
-        own_wrbuf_xtpls wrbuf ∅ ∧ ⌜int.nat tid = ts⌝
+        own_txn_impl txn wrbuf ts' γ ∗
+        own_wrbuf_xtpls wrbuf ∅ ∧ ⌜int.nat tid = ts'⌝
     }}}.
 Proof.
   iIntros "!>" (Φ) "Htxn HAU".
@@ -34,7 +34,7 @@ Proof.
   iModIntro.
   iExists ts.
   iFrame "Hts".
-  iIntros "[%n H]".
+  iIntros "%n [H %Hlt]".
   iMod ("HAUC" with "[H]") as "HΦ"; first eauto with iFrame.
   iIntros "!>" (tid) "[Hactive %HtidNZ]".
 
@@ -53,8 +53,9 @@ Proof.
   wp_pures.
 
   iModIntro.
-  iApply "HΦ".
-  eauto 20 with iFrame.
+  iApply "HΦ". iFrame "HwrbufRP". iSplitL; last done.
+  repeat iExists _. iFrame "∗#".
+  iSplit; done.
 Qed.
 
 End program.
